WIP: defining simulation

theories/simulation.v
@@ -1,108 +1,84 @@
-From stbor Require Import lang notation steps.
 From Paco Require Import paco.
+From stbor Require Export properties.
 
-Class Terminal A := terminal : A → Prop.
-Existing Class terminal.
+(** Configuration simulation *)
 
-Definition epxr_terminal' (e: expr) : Prop := is_Some (to_val e).
-Instance expr_terminal : Terminal expr := epxr_terminal'.
+Notation SIM_CFG := (relation (cfg bor_lang))%type.
+
+(* TODO: do we need observations more than a singleton list? *)
+(* TODO: de we need to relax the observation relation? *)
+Definition _sim (sim: SIM_CFG) (ρ1_src ρ1_tgt : cfg bor_lang) : Prop :=
+  (* Wf ρ1_src → Wf ρ1_tgt → *)
+  ∀ σ1_src σ1_tgt,
+  (* σ1_src, σ1_tgt are new states by other threads' interferences *)
+  Wf σ1_src → Wf σ1_tgt →
+  future_state ρ1_src.2 σ1_src → future_state ρ1_tgt.2 σ1_tgt →
+  (* σ1_src, σ1_tgt are related *)
+  sim_state σ1_src σ1_tgt →
+  (* (1) If `ρ1_tgt` is terminal, then `ρ1_src` terminates with τ steps. *)
+  (terminal ρ1_tgt.1 → ∃ T2_src σ2_src,
+      rtc τstep (ρ1_src.1, σ1_src) (T2_src, σ2_src) ∧
+      sim_state σ2_src σ1_tgt ∧ terminal T2_src) ∧
+  (* (2) If `ρ1_tgt` steps to `ρ2_tgt` with observation o, then exists `ρ2_src`
+         s.t. `ρ1_src` steps to `ρ2_src` with observation o AND
+         ρ2_src and ρ2_tgt related by sim. *)
+  (∀ ρ2_tgt tid_tgt o, one_step (ρ1_tgt.1, σ1_tgt) tid_tgt o ρ2_tgt →
+      ∃ ρ2_src tid_src, one_step (ρ1_src.1, σ1_src) tid_src o ρ2_src ∧
+      sim_state ρ1_src.2 ρ2_tgt.2 ∧ sim ρ2_src ρ2_tgt).
+
+Lemma _sim_monotone : monotone2 _sim.
+Proof.
+  intros ρ1_src ρ1_tgt r r' TS LE σ1_src σ1_tgt WF1 WF2 FT1 FT2 SS.
+  destruct (TS _ _ WF1 WF2 FT1 FT2 SS) as [TERM STEP]. split; [done|].
+  intros ρ2_tgt tid o ONE.
+  destruct (STEP _ _ _ ONE) as [ρ2_src [tid_src [ONE_src [SS2 Hr]]]].
+  exists ρ2_src, tid_src. do 2 (split; [done|]). by apply LE.
+Qed.
+Hint Resolve _sim_monotone: paco.
+
+(** The actual simulation *)
+Definition sim: SIM_CFG := paco2 _sim bot2.
 
 (** Thread simulation *)
-Definition SIM_EXPR := relation expr.
-Definition SIM_THREAD := SIM_EXPR → expr → state → expr → state → Prop.
-
-(* TODO: we are ignoring fork *)
-(* thread τ-step has no observation. *)
-Inductive thread_τstep (eσ1 eσ2: expr * state) : Prop :=
-| ThreadTauStep (STEP: prim_step eσ1.1 eσ1.2 [] eσ2.1 eσ2.2 []).
-Inductive thread_onestep eσ1 o eσ2 : Prop :=
-| ThreadOneStep eσ1'
-    (TAU_STEP: rtc thread_τstep eσ1 eσ1')
-    (ONE_STEP: prim_step eσ1'.1 eσ1'.2 [o] eσ2.1 eσ2.2 []).
+Notation SIM_EXPR := (relation expr)%type.
+Notation SIM_THREAD := (SIM_EXPR → expr → state → expr → state → Prop)%type.
 
 Definition _sim_thread (sim_thread: SIM_THREAD) (sim_terminal: SIM_EXPR)
-  (e1_src: expr) (σ1_src: state) (e1_tgt: expr) (σ1_tgt: state) : Prop :=
-  (* assuming wellformedness *)
+  (e1_src: expr) (σ0_src: state) (e1_tgt: expr) (σ0_tgt: state) : Prop :=
+  (* Wf ρ1_src → Wf ρ1_tgt → *)
+  ∀ σ1_src σ1_tgt,
+  (* σ1_src, σ1_tgt are new states by other threads' interferences *)
   Wf σ1_src → Wf σ1_tgt →
-  (* TODO: state relations σ1_src & σ1_tgt → *)
+  future_state σ0_src σ1_src → future_state σ0_tgt σ1_tgt →
+  (* σ1_src, σ1_tgt are related *)
+  sim_state σ1_src σ1_tgt →
   (* (1) If `e1_tgt` is terminal, then `e1_src` terminates with τ steps *)
   (terminal e1_tgt → ∃ e2_src σ2_src,
     rtc thread_τstep (e1_src, σ1_src) (e2_src, σ2_src) ∧
-    terminal e2_src ∧ sim_terminal e2_src e1_tgt
-    (* ∧ state relations: σ2_src & σ1_tgt *)) ∧
+    sim_state σ2_src σ1_tgt ∧
+    terminal e2_src ∧ sim_terminal e2_src e1_tgt) ∧
   (* (2) If `(e1_tgt, σ1_tgt)` steps to `(e2_tgt, σ2_tgt)` with observation o,
          then exists `(e2_src, σ2_src)`
          s.t. `(e1_src, σ1_src)` steps to `(e2_src, σ2_src)` with observation o *)
   (∀ e2_tgt σ2_tgt o, thread_onestep (e1_tgt, σ1_tgt) o (e2_tgt, σ2_tgt)
     → ∃ e2_src σ2_src,
       thread_onestep (e1_src, σ1_src) o (e2_src, σ2_src) ∧
-      sim_thread sim_terminal e2_src σ2_src e2_tgt σ2_tgt
-      (* TODO: state relations σ2_src & σ2_tgt → *)).
+      sim_state σ2_src σ2_tgt ∧
+      sim_thread sim_terminal e2_src σ2_src e2_tgt σ2_tgt).
 
 Lemma _sim_thread_monotone : monotone5 _sim_thread.
 Proof.
-  intros re e1_src σ1_src e1_tgt σ1_tgt r r' TS LE WF1 WF2.
-  destruct (TS WF1 WF2) as [TERM STEP]. split; [done|].
+  intros re ???? r r' TS LE σ1_src σ1_tgt WF1 WF2 FT1 FT2 SS.
+  destruct (TS _ _ WF1 WF2 FT1 FT2 SS) as [TERM STEP]. split; [done|].
   intros e2_tgt σ2_tgt o ONE.
-  destruct (STEP _ _ _ ONE) as (e2_src & σ2_src & ONE_src & Hr).
-  exists e2_src, σ2_src. split; [done|by apply LE].
+  destruct (STEP _ _ _ ONE) as (e2_src & σ2_src & ONE_src & SS' & Hr).
+  exists e2_src, σ2_src. do 2 (split; [done|]). by apply LE.
 Qed.
 Hint Resolve _sim_thread_monotone: paco.
 
 Definition sim_thread: SIM_THREAD := paco5 _sim_thread bot5.
 
-(** Configuration simulation *)
-Implicit Type (ρ: cfg bor_lang).
-
-Definition cfg_terminal' ρ : Prop := ∀ e, e ∈ ρ.1 → terminal e.
-Instance cfg_terminal : Terminal (cfg bor_lang) := cfg_terminal'.
-
-(* This duplicates iris.program_logic.language to expose a thread id *)
-Inductive step ρ1 tid κ ρ2 : Prop :=
-| StepAtomic e1 σ1 e2 σ2 efs t1 t2 :
-   ρ1 = (t1 ++ e1 :: t2, σ1) →
-   ρ2 = (t1 ++ e2 :: t2 ++ efs, σ2) →
-   prim_step e1 σ1 κ e2 σ2 efs →
-   tid = length t1 →
-   step ρ1 tid κ ρ2.
-
-(* τ-step has no observation and ignore tid. *)
-Inductive τstep ρ1 ρ2 : Prop :=
-| TauStep tid (STEP: step ρ1 tid [] ρ2).
-
-(* One true step can be led by some τ-steps. *)
-Inductive one_step ρ1 tid o ρ2 : Prop :=
-| OneStep ρ1' (TAU_STEP: rtc τstep ρ1 ρ1') (ONE_STEP: step ρ1' tid [o] ρ2).
-
-(* TODO: do we need observations more than a singleton list? *)
-(* TODO: de we need to relax the observation relation? *)
-Definition _sim (sim: relation (cfg bor_lang)) (ρ1_src ρ1_tgt : cfg bor_lang)
-  : Prop :=
-  (* assuming wellformedness *)
-  Wf ρ1_src.2 → Wf ρ1_tgt.2 →
-  (* TODO: state relations ρ1_src & ρ1_tgt → *)
-  (* (1) If `ρ1_tgt` is terminal, then `ρ1_src` terminates with τ steps *)
-  (terminal ρ1_tgt → ∃ ρ2_src, rtc τstep ρ1_src ρ2_src ∧ terminal ρ2_src
-      (* ∧ state relations: ρ2_src & ρ1_tgt *)) ∧
-  (* (2) If `ρ1_tgt` steps to `ρ2_tgt` with observation o, then exists `ρ2_src`
-         s.t. `ρ1_src` steps to `ρ2_src` with observation o *)
-  (∀ ρ2_tgt tid o, one_step ρ1_tgt tid o ρ2_tgt → ∃ ρ2_src,
-      one_step ρ1_src tid o ρ2_src ∧ sim ρ2_src ρ2_tgt
-      (* TODO: state relations ρ1_src & ρ1_tgt → *)).
-
-Lemma _sim_monotone : monotone2 _sim.
-Proof.
-  intros ρ1_src ρ1_tgt r r' TS LE WF1 WF2.
-  destruct (TS WF1 WF2) as [TERM STEP]. split; [done|].
-  intros ρ2_tgt tid o ONE. destruct (STEP _ _ _ ONE) as [ρ2_src [ONE_src Hr]].
-  exists ρ2_src. split; [done|by apply LE].
-Qed.
-Hint Resolve _sim_monotone: paco.
-
-(** The actual simulation *)
-Definition sim: relation (cfg bor_lang) := paco2 _sim bot2.
-
-(** Composition (probably not needed: composing disjoint configuration preserves
+(** Composition : composing disjoint configuration preserves
   configuration simulation *)
 
 (** Compatibility: language constructs preserve thread/configuration simulation *)
