theories/properties.v
@@ -1,0 +1,91 @@
+From stbor Require Export lang notation.
+
+(** Wellformedness *)
+Class Wellformed A := Wf : A → Prop.
+Existing Class Wf.
+
+Definition wf_mem_bor (h: mem) (clock: time) :=
+  ∀ l l' bor, h !! l = Some (LitV (LitLoc l' bor)) → bor <b clock.
+
+Definition frozen_lt (stk: bstack) (clk: time) :=
+  match frozen_since stk with
+  | Some t => (t < clk)%nat
+  | None => True
+  end.
+Definition wf_stack_frozen (α: bstacks) (clock: time) :=
+  ∀ l stack, α !! l = Some stack → frozen_lt stack clock.
+
+Definition stack_item_included (stk: bstack) (β: barriers) (clock: time) :=
+  ∀ si, si ∈ stk.(borrows) → match si with
+                              | Uniq t => (t < clock)%nat
+                              | FnBarrier c => is_Some (β !! c)
+                              | _ => True
+                              end.
+Definition wf_stack_item (α: bstacks) (β: barriers) (clock: time) :=
+  ∀ l stack, α !! l = Some stack → stack_item_included stack β clock.
+Definition borrow_barrier_Some (β: barriers) kind : Prop :=
+  match kind with FnEntry c => is_Some (β !! c) | _ => True end.
+Definition wf_non_empty (α: bstacks) :=
+   ∀ l stack, α !! l = Some stack → stack.(borrows) ≠ [].
+
+Record state_wf' σ := {
+  state_wf_dom : dom (gset loc) σ.(cheap) ≡ dom (gset loc) σ.(cstk);
+  state_wf_mem_bor : wf_mem_bor σ.(cheap) σ.(cclk);
+  state_wf_stack_frozen : wf_stack_frozen σ.(cstk) σ.(cclk);
+  state_wf_stack_item : wf_stack_item σ.(cstk) σ.(cbar) σ.(cclk);
+  state_wf_non_empty : wf_non_empty σ.(cstk);
+}.
+
+Instance state_wf : Wellformed state :=  state_wf'.
+
+Implicit Type (ρ: cfg bor_lang).
+
+(* TODO: this may need strengthening *)
+Definition cfg_wf' ρ : Prop := Wf ρ.2.
+Instance cfg_wf : Wellformed (cfg bor_lang) :=  cfg_wf'.
+
+(** Terminal states *)
+Class Terminal A := terminal : A → Prop.
+Existing Class terminal.
+
+Definition epxr_terminal' (e: expr) : Prop := is_Some (to_val e).
+Instance expr_terminal : Terminal expr := epxr_terminal'.
+Definition threads_terminal' (el: list expr) := ∀ e, e ∈ el → terminal e.
+Instance threads_terminal : Terminal (list expr) := threads_terminal'.
+Definition cfg_terminal' ρ : Prop := terminal ρ.1.
+Instance cfg_terminal : Terminal (cfg bor_lang) := cfg_terminal'.
+
+(** Thread steps *)
+(* TODO: we are ignoring fork *)
+(* τ-step has no observation. *)
+Inductive thread_τstep (eσ1 eσ2: expr * state) : Prop :=
+| ThreadTauStep (STEP: prim_step eσ1.1 eσ1.2 [] eσ2.1 eσ2.2 []).
+(* One true step can be led by some τ-steps. *)
+Inductive thread_onestep eσ1 o eσ2 : Prop :=
+| ThreadOneStep eσ1'
+    (TAU_STEP: rtc thread_τstep eσ1 eσ1')
+    (ONE_STEP: prim_step eσ1'.1 eσ1'.2 [o] eσ2.1 eσ2.2 []).
+
+(** Configuration (threadpool) steps *)
+(* This duplicates iris.program_logic.language in order to expose a thread id *)
+Inductive step ρ1 tid κ ρ2 : Prop :=
+| StepAtomic e1 σ1 e2 σ2 efs t1 t2 :
+   ρ1 = (t1 ++ e1 :: t2, σ1) →
+   ρ2 = (t1 ++ e2 :: t2 ++ efs, σ2) →
+   prim_step e1 σ1 κ e2 σ2 efs →
+   tid = length t1 →
+   step ρ1 tid κ ρ2.
+
+(* τ-step has no observation and ignore tid. *)
+Inductive τstep ρ1 ρ2 : Prop :=
+| CfgTauStep tid (STEP: step ρ1 tid [] ρ2).
+(* One true step can be led by some τ-steps. *)
+Inductive one_step ρ1 tid o ρ2 : Prop :=
+| CfgOneStep ρ1' (TAU_STEP: rtc τstep ρ1 ρ1') (ONE_STEP: step ρ1' tid [o] ρ2).
+
+(** Future states,  by interference *)
+(* TODO: fix this *)
+Definition future_state : relation state := λ σ1 σ2, σ1 = σ2.
+(** State simulation *)
+(* TODO: fix this *)
+Definition sim_state : relation state := λ σ1 σ2, σ1 = σ2.
